update SmallStep.v

programming_language_foundations/SmallStep.v
@@ -765,3 +765,293 @@ Module Combined.
 End Combined.
 
 (* Small-Step Imp *)
+
+Inductive aval : aexp -> Prop :=
+| av_num : forall n, aval (ANum n).
+
+Reserved Notation " t '/' st '-->a' t' "
+         (at level 40, st at level 39).
+
+Inductive astep : state -> aexp -> aexp -> Prop :=
+| AS_Id : forall st i,
+    AId i / st -->a ANum (st i)
+| AS_Plus1 : forall st a1 a1' a2,
+    a1 / st -->a a1' ->
+    (APlus a1 a2) / st -->a (APlus a1' a2)
+| AS_Plus2 : forall st v1 a2 a2',
+    aval v1 ->
+    a2 / st -->a a2' ->
+    (APlus v1 a2) / st -->a (APlus v1 a2')
+| AS_Plus : forall st n1 n2,
+    APlus (ANum n1) (ANum n2) / st -->a ANum (n1 + n2)
+| AS_Minus1 : forall st a1 a1' a2,
+    a1 / st -->a a1' ->
+    (AMinus a1 a2) / st -->a (AMinus a1' a2)
+| AS_Minus2 : forall st v1 a2 a2',
+    aval v1 ->
+    a2 / st -->a a2' ->
+    (AMinus v1 a2) / st -->a (AMinus v1 a2')
+| AS_Minus : forall st n1 n2,
+    (AMinus (ANum n1) (ANum n2)) / st -->a (ANum (minus n1 n2))
+| AS_Mult1 : forall st a1 a1' a2,
+    a1 / st -->a a1' ->
+    (AMult a1 a2) / st -->a (AMult a1' a2)
+| AS_Mult2 : forall st v1 a2 a2',
+    aval v1 ->
+    a2 / st -->a a2' ->
+    (AMult v1 a2) / st -->a (AMult v1 a2')
+| AS_Mult : forall st n1 n2,
+    (AMult (ANum n1) (ANum n2)) / st -->a (ANum (mult n1 n2))
+where " t '/' st '-->a' t' " := (astep st t t').
+
+Reserved Notation " t '/' st '-->b' t' "
+         (at level 40, st at level 39).
+
+Inductive bstep : state -> bexp -> bexp -> Prop :=
+| BS_Eq1 : forall st a1 a1' a2,
+    a1 / st -->a a1' ->
+    (BEq a1 a2) / st -->b (BEq a1' a2)
+| BS_Eq2 : forall st v1 a2 a2',
+    aval v1 ->
+    a2 / st -->a a2' ->
+    (BEq v1 a2) / st -->b (BEq v1 a2')
+| BS_Eq : forall st n1 n2,
+    (BEq (ANum n1) (ANum n2)) / st -->b
+             (if (n1 =? n2) then BTrue else BFalse)
+| BS_LtEq1 : forall st a1 a1' a2,
+    a1 / st -->a a1' ->
+    (BLe a1 a2) / st -->b (BLe a1' a2)
+| BS_LtEq2 : forall st v1 a2 a2',
+    aval v1 ->
+    a2 / st -->a a2' ->
+    (BLe v1 a2) / st -->b (BLe v1 a2')
+| BS_LtEq : forall st n1 n2,
+    (BLe (ANum n1) (ANum n2)) / st -->b
+             (if (n1 <=? n2) then BTrue else BFalse)
+| BS_NotStep : forall st b1 b1',
+    b1 / st -->b b1' ->
+    (BNot b1) / st -->b (BNot b1')
+| BS_NotTrue : forall st,
+    (BNot BTrue) / st -->b BFalse
+| BS_NotFalse : forall st,
+    (BNot BFalse) / st -->b BTrue
+| BS_AndTrueStep : forall st b2 b2',
+    b2 / st -->b b2' ->
+    (BAnd BTrue b2) / st -->b (BAnd BTrue b2')
+| BS_AndStep : forall st b1 b1' b2,
+    b1 / st -->b b1' ->
+    (BAnd b1 b2) / st -->b (BAnd b1' b2)
+| BS_AndTrueTrue : forall st,
+    (BAnd BTrue BTrue) / st -->b BTrue
+| BS_AndTrueFalse : forall st,
+    (BAnd BTrue BFalse) / st -->b BFalse
+| BS_AndFalse : forall st b2,
+    (BAnd BFalse b2) / st -->b BFalse
+
+where " t '/' st '-->b' t' " := (bstep st t t').
+
+Reserved Notation " t '/' st '-->' t' '/' st' "
+         (at level 40, st at level 39, t' at level 39).
+
+Open Scope imp_scope.
+Inductive cstep : (com * state) -> (com * state) -> Prop :=
+| CS_AssStep : forall st i a a',
+    a / st -->a a' ->
+    (i ::= a) / st --> (i ::= a') / st
+| CS_Ass : forall st i n,
+    (i ::= (ANum n)) / st --> SKIP / (i !-> n; st)
+| CS_SeqStep : forall st c1 c1' st' c2,
+    c1 / st --> c1' / st' ->
+    (c1 ;; c2) / st --> (c1' ;; c2) / st'
+| CS_SeqFinish : forall st c2,
+    (SKIP ;; c2) / st --> c2 / st
+| CS_IfStep : forall st b b' c1 c2,
+    b / st -->b b' ->
+    TEST b THEN c1 ELSE c2 FI / st
+    -->
+    (TEST b' THEN c1 ELSE c2 FI) / st
+| CS_IfTrue : forall st c1 c2,
+    TEST BTrue THEN c1 ELSE c2 FI / st --> c1 / st
+| CS_IfFalse : forall st c1 c2,
+    TEST BFalse THEN c1 ELSE c2 FI / st --> c2 / st
+| CS_While : forall st b c1,
+    WHILE b DO c1 END / st
+    -->
+    (TEST b THEN c1;; WHILE b DO c1 END ELSE SKIP FI) / st
+where " t '/' st '-->' t' '/' st' " := (cstep (t,st) (t',st')).
+
+Close Scope imp_scope.
+
+Module CImp.
+  
+  Inductive com : Type :=
+  | CSkip : com
+  | CAss : string -> aexp -> com
+  | CSeq : com -> com -> com
+  | CIf : bexp -> com -> com -> com
+  | CWhile : bexp -> com -> com
+  | CPar : com -> com -> com. (* <--- NEW *)
+
+  Notation "'SKIP'" :=
+    CSkip.
+  Notation "x '::=' a" :=
+    (CAss x a) (at level 60).
+  Notation "c1 ;; c2" :=
+    (CSeq c1 c2) (at level 80, right associativity).
+  Notation "'WHILE' b 'DO' c 'END'" :=
+    (CWhile b c) (at level 80, right associativity).
+  Notation "'TEST' b 'THEN' c1 'ELSE' c2 'FI'" :=
+    (CIf b c1 c2) (at level 80, right associativity).
+  Notation "'PAR' c1 'WITH' c2 'END'" :=
+    (CPar c1 c2) (at level 80, right associativity).
+  
+  Inductive cstep : (com * state) -> (com * state) -> Prop :=
+  (* Old part *)
+  | CS_AssStep : forall st i a a',
+      a / st -->a a' ->
+      (i ::= a) / st --> (i ::= a') / st
+  | CS_Ass : forall st i n,
+      (i ::= (ANum n)) / st --> SKIP / (i !-> n ; st)
+  | CS_SeqStep : forall st c1 c1' st' c2,
+      c1 / st --> c1' / st' ->
+      (c1 ;; c2) / st --> (c1' ;; c2) / st'
+  | CS_SeqFinish : forall st c2,
+      (SKIP ;; c2) / st --> c2 / st
+  | CS_IfStep : forall st b b' c1 c2,
+      b /st -->b b' ->
+          (TEST b THEN c1 ELSE c2 FI) / st 
+      --> (TEST b' THEN c1 ELSE c2 FI) / st
+  | CS_IfTrue : forall st c1 c2,
+      (TEST BTrue THEN c1 ELSE c2 FI) / st --> c1 / st
+  | CS_IfFalse : forall st c1 c2,
+      (TEST BFalse THEN c1 ELSE c2 FI) / st --> c2 / st
+  | CS_While : forall st b c1,
+          (WHILE b DO c1 END) / st 
+      --> (TEST b THEN (c1;; (WHILE b DO c1 END)) ELSE SKIP FI) / st
+    (* New part: *)
+  | CS_Par1 : forall st c1 c1' c2 st',
+      c1 / st --> c1' / st' ->
+      (PAR c1 WITH c2 END) / st --> (PAR c1' WITH c2 END) / st'
+  | CS_Par2 : forall st c1 c2 c2' st',
+      c2 / st --> c2' / st' ->
+      (PAR c1 WITH c2 END) / st --> (PAR c1 WITH c2' END) / st'
+  | CS_ParDone : forall st,
+      (PAR SKIP WITH SKIP END) / st --> SKIP / st
+  where " t '/' st '-->' t' '/' st' " := (cstep (t,st) (t',st')).
+  
+  Definition cmultistep := multi cstep.
+  
+  Notation " t '/' st '-->*' t' '/' st' " :=
+    (multi cstep (t,st) (t',st'))
+      (at level 40, st at level 39, t' at level 39).
+
+  Definition par_loop : com :=
+  PAR
+    Y ::= 1
+  WITH
+    WHILE Y = 0 DO
+      X ::= X + 1
+    END
+  END.
+
+  Example par_loop_example_0 :
+    exists st',
+      par_loop / empty_st -->* SKIP / st'
+      /\ st' X = 0.
+  Proof.
+    unfold par_loop.
+    eexists. split.
+    - eapply (multi_step cstep).
+      + apply CS_Par1. apply CS_Ass.
+      + eapply (multi_step cstep).
+        * apply CS_Par2. apply CS_While.
+        * eapply (multi_step cstep).
+          { apply CS_Par2. apply CS_IfStep. apply BS_Eq1. apply AS_Id. }
+          { rewrite t_update_eq. eapply (multi_step cstep).
+            { apply CS_Par2. apply CS_IfStep. apply BS_Eq. }
+            { simpl. eapply (multi_step cstep).
+              { apply CS_Par2. apply CS_IfFalse. }
+              { eapply (multi_step cstep).
+                { apply CS_ParDone. }
+                { apply (multi_refl cstep). }
+              }
+            }
+          }
+    - rewrite t_update_neq.
+      + unfold empty_st. apply t_apply_empty.
+      + intro. inversion H.
+  Qed.
+
+  Example par_loop_example_2 :
+    exists st', par_loop / empty_st -->* SKIP / st'
+                /\ st' X = 2.
+  Proof.
+    eapply ex_intro. split.
+    unfold par_loop.
+    eapply multi_step.
+    - apply CS_Par2. apply CS_While.
+    - eapply multi_step.
+      + apply CS_Par2. apply CS_IfStep. apply BS_Eq1. apply AS_Id.
+      + eapply multi_step. apply CS_Par2. unfold empty_st. rewrite t_apply_empty.
+        apply CS_IfStep. apply BS_Eq. simpl. eapply multi_step.
+        * apply CS_Par2. apply CS_IfTrue.
+        * eapply multi_step.
+          { apply CS_Par2. apply CS_SeqStep. apply CS_AssStep. apply AS_Plus1. apply AS_Id. }
+          { rewrite t_apply_empty. eapply multi_step.
+            { apply CS_Par2. apply CS_SeqStep. apply CS_AssStep. apply AS_Plus. }
+            { simpl. eapply multi_step.
+              { apply CS_Par2. apply CS_SeqStep. apply CS_Ass. }
+              { eapply multi_step.
+                { apply CS_Par2. apply CS_SeqFinish. }
+                { eapply multi_step.
+                  { apply CS_Par2. apply CS_While. }
+                  { eapply multi_step.
+                    { apply CS_Par2. apply CS_IfStep. apply BS_Eq1. apply AS_Id. }
+                    { eapply multi_step. apply CS_Par2. rewrite t_update_neq.
+                      { unfold empty_st. rewrite t_apply_empty.
+                        apply CS_IfStep. apply BS_Eq. }
+                      { intro. inversion H. }
+                      simpl. eapply multi_step.
+                      { apply CS_Par2. apply CS_IfTrue. }
+                      { eapply multi_step.
+                        { apply CS_Par2. apply CS_SeqStep. apply CS_AssStep. apply AS_Plus1. apply AS_Id. }
+                        { rewrite t_update_eq. eapply multi_step.
+                          { apply CS_Par2. apply CS_SeqStep. apply CS_AssStep. apply AS_Plus. }
+                          { simpl. eapply multi_step.
+                            { apply CS_Par2. apply CS_SeqStep. apply CS_Ass. }
+                            { eapply multi_step.
+                              { apply CS_Par2. apply CS_SeqFinish. }
+                              { eapply multi_step.
+                                { apply CS_Par1. apply CS_Ass. }
+                                { eapply multi_step.
+                                  { apply CS_Par2. apply CS_While. }
+                                  { eapply multi_step.
+                                    { apply CS_Par2. apply CS_IfStep. apply BS_Eq1. apply AS_Id. }
+                                    { rewrite t_update_eq. eapply multi_step.
+                                      { apply CS_Par2. apply CS_IfStep. apply BS_Eq. }
+                                      { eapply multi_step.
+                                        { simpl. apply CS_Par2. apply CS_IfFalse. }
+                                        { eapply multi_step.
+                                          { apply CS_ParDone. }
+                                          { apply (multi_refl cstep). }
+                                        }
+                                      }
+                                    }
+                                  }
+                                }
+                              }
+                            }
+                          }
+                        }
+                      }
+                    }
+                  }
+                }
+              }
+            }
+          }
+    - rewrite t_update_neq.
+      + rewrite t_update_eq. reflexivity.
+      + intro. inversion H.
+  Qed.
+  
